Wavelet/Determinacy/Confluence.lean
@@ -643,7 +643,7 @@ theorem proc_indexed_interp_guarded_strong_confl_at
             have := haff.atom_inputs_disjoint
               ⟨i₁, by assumption⟩ ⟨i₂, by assumption⟩ (by simp [heq_ij])
             simp [hget₁, hget₂, AtomicProc.inputs] at this
-            have := pop_vals_pop_vals_disj_preserves_pairwise hdisj this hpop₁ hpop₂
+            have := pop_vals_pop_vals_disj_preserves_pairwise hdisj.2 this hpop₁ hpop₂
             apply this (.inr (opSpec.pre op₁ inputVals₁)) (.inr (opSpec.pre op₂ inputVals₂))
             all_goals simp)
         replace ⟨s', hstep₁', hstep₂'⟩ := h
@@ -782,7 +782,7 @@ theorem proc_interp_guarded_strong_confl_at
             -- apply PCM.eq_congr_disj htok₁ htok₂
             have := haff.atom_inputs_disjoint ⟨i, hi⟩ ⟨j, hj⟩ (by simp [heq_ij])
             simp [hget_i, hget_j, AtomicProc.inputs] at this
-            have := pop_vals_pop_vals_disj_preserves_pairwise hdisj this hpop₁ hpop₂
+            have := pop_vals_pop_vals_disj_preserves_pairwise hdisj.2 this hpop₁ hpop₂
             -- have := this (.inr _) (.inr _)
             apply this (.inr (opSpec.pre op₁ inputVals₁)) (.inr (opSpec.pre op₂ inputVals₂))
             all_goals simp)
